Bigint impl first iteration (#9)
* Use Dockerfile from main

* implement BigInteger partially

* update Makefile

* Update BigInt implementation

* Update BigInt implementation

* implemented sub_with_borrow

* Update BigInt implementation

* Change `panic` for `unimplemented`

* Partially implement `mul` for `BigInt`

* Update `mul` method for `BigInt`

* Update BigInt implementation

* Refactor BigInt implementation

* Update Cargo.toml

* base steps to finish bigint; tests are working with some decommenting

* make base version of BigInt working with lean frontend

* implemented is_even proof

* added overflow proofs from Shu

* refactored proofs a little bit

* deleted temp build files

* updated lean version to make it buildable

---------

Co-authored-by: dbsc <andredbsc@gmail.com>
Co-authored-by: dbsc <69024997+dbsc@users.noreply.github.com>
Co-authored-by: unknown <remi.djabiri@gmail.com>

src/main.rs
@@ -1,4 +1,0 @@
-mod arithmetics;
-
-fn main() {
-}
