test/lean/Proofs/Addition.lean
@@ -1,5 +1,4 @@
-import Test.Funs
-import Base
+import Common.Base
 
 open Primitives
 open Result
@@ -10,206 +9,10 @@ namespace biginteger
 
 attribute [-simp] Bool.exists_bool
 
-def valImpl (l : List U64) : Int :=
-  match l with
-  | a::b => a.val + (valImpl b) * (2 ^ 64)
-  | [] => 0
-
-lemma valImpl_ge_zero (l : List U64) : valImpl l ≥ 0 := by
-  unfold valImpl
-  match l with
-  | a::b => {
-    have ha : 0 ≤ a.val := by scalar_tac
-    have hb : 0 ≤ valImpl b * 2 ^ 64 := by simp[valImpl_ge_zero]
-    have hc := Int.add_le_add ha hb
-    simp at hc
-    simp [*]
-  }
-  | [] => simp
-
-@[simp]
-lemma tmp : Inhabited U64 := by
-  constructor
-  apply 0#u64
-
--- Biggest part by Son Ho
-lemma BigInt.update_eq (l : List U64) (i : Int) (x : U64)
-  (h0 : 0 ≤ i) (h1 : i < l.len) :
-  valImpl (l.update i x) = valImpl l + (x - l.index i) * ((2 ^ 64) ^ i.toNat) := by
-  match l with
-  | [] =>
-    -- Contradiction: 0 ≤ i ∧ i < 0
-    simp at h1
-    scalar_tac
-  | h :: tl =>
-    simp at h1
-    if i = 0 then
-      simp [*] -- By writing [*] I'm using the hypothesis i = 0
-      unfold valImpl
-      scalar_tac
-    else
-      have hnz : i ≠ 0 := by scalar_tac
-      -- This uses update_nzero_cons and index_nzero_cons
-      simp only [h1, hnz, ne_eq, not_false_eq_true, List.update_nzero_cons, List.index_nzero_cons] -- By writing [*] I'm using the hypothesis i ≠ 0
-      unfold valImpl
-      -- Recursive call
-      have heq := update_eq tl (i - 1) x (by scalar_tac) (by scalar_tac)
-      rw [heq]
-      rw [add_mul]
-      simp only [Int.pred_toNat]
-      have hexpr : ((2: Int) ^ 64) ^ (Int.toNat i - 1) * 2 ^ 64 = (2 ^ 64) ^ Int.toNat i := by {
-        rw [←pow_mul]
-        rw [←pow_add]
-        rw [←pow_mul]
-        rw [Nat.mul_sub_left_distrib]
-        rw [←Nat.sub_add_comm]
-        simp [*]
-        have hgone : i ≥ 1 := by scalar_tac
-        simp [hgone, *]
-      }
-      simp only [mul_assoc]
-      rw [hexpr]
-      simp [add_assoc]
-
-
-@[simp] lemma BigInt.len_spec
-  (N : Usize) (self : biginteger.BigInt N) :
-  (self.val).len = N.val := by
-  have h := self.property
-  rw [List.len_eq_length]
-  apply h
-
-def BigInt.val {N : Usize} (x : biginteger.BigInt N) : Int := valImpl x.v
-
-def BigInt.mod_value (n : Int) : Int := (U64.max + 1) ^ (Int.toNat n)
-
-def BigInt.max_value (n : Int) : Int := BigInt.mod_value n - 1
-
-lemma BigInt.mod_value_add_one (n : Int) (hn : 0 ≤ n) : BigInt.mod_value n * (2 ^ 64) = BigInt.mod_value (n + 1) := by
-  rw [BigInt.mod_value]
-  rw [BigInt.mod_value]
-  rw [U64.max]
-  simp
-  -- rw [mul_comm]
-  rw [←pow_succ]
-  -- simp []
-  have hf := Int.toNat_add_nat hn 1
-  rw [←hf]
-  simp
-
-lemma valImpl_lt_mod (l : List U64) : valImpl l < BigInt.mod_value l.len := by
-  unfold valImpl
-  match h : l with
-  | a::b => {
-    simp only [List.len_cons, gt_iff_lt]
-    have ha := valImpl_lt_mod b
-    have hb : a.val < 2 ^ 64 := by scalar_tac
-    have hc := Int.le_sub_one_of_lt ha
-    have hd : 1 + b.len = b.len + 1 := by scalar_tac
-    have hf : (0 : Int) ≤ 2 ^ 64 := by simp
-    have hg := Int.mul_le_mul_of_nonneg_right hc hf
-    simp only [Int.sub_mul] at hg
-    simp only [one_mul] at hg
-    have hh := add_lt_add_of_le_of_lt hg hb
-    simp only [sub_add_cancel] at hh
-    rw [Int.add_comm] at hh
-    rw [hd]
-    rw [←BigInt.mod_value_add_one]
-    simp only [hh]
-    scalar_tac
-  }
-  | [] => {
-    simp
-    unfold BigInt.mod_value
-    simp
-  }
-
-
-lemma BigInt.val_lt_mod (N : Usize) (bn : Array U64 N) : valImpl bn.val < BigInt.mod_value N.val := by
-  have hi := valImpl_lt_mod bn.val
-  have he := bn.property
-  simp [*, List.len_eq_length] at hi
-  simp [*]
-
 theorem adc_for_add_with_carry_spec (a : U64) (b : U64) (carry : U8) :
-  ∃ new_carry r, biginteger.arithmetic.adc_for_add_with_carry a b carry = .ok (new_carry, r) ∧
+  ∃ new_carry r, biginteger.arithmetic.adc_for_add_with_carry a b carry = .ok (new_carry, r) ∧ 
   new_carry = (a.val + b.val + carry.val) / (2 ^ 64) ∧
   r = (a.val + b.val + carry.val) % 2 ^ 64 := by sorry
-
-
-lemma BigInt.ha_0_val (N: Usize) (bi : Array U64 N) : N = 0#usize → valImpl bi.val = 0 :=
-by {
-      unfold valImpl;
-      intro hN;
-      have h := bi.property;
-      match hq0 : bi.val with
-        | [] => scalar_tac;
-        | hd :: tl => {
-            simp [BigInt.len_spec, hN, List.len_eq_length, *] at h; scalar_tac;
-        }
-  }
-
--- lemma BigInt.h_1_val (N: Usize) (bi : BigInt N) : N = 1#usize → valImpl (Array.v bi) = (Array.v bi).index 0#usize.val  :=
--- by {
---         simp [BigInt.val];
---         unfold valImpl;
---         have h := BigInt.len_spec N bi;
---         match hq0 : bi.val with
---         | [] => simp [List.len_nil, Usize.ofInt_val_eq, hq0] at h; scalar_tac;
---         | hd :: tl => {
---           simp []
---           unfold valImpl
---           match hq1 : tl with
---           | [] => simp [];
---           | hd::tl2 => simp [*, List.len_eq_length] at h; scalar_tac;
---         }
---       }
-
-lemma BigInt.slice_eq (l : List U64) (i : Int) (N : Int)
-  (h0 : 0 ≤ i) (h1 : i < N) (h2 : N ≤ l.len) :
-  valImpl (l.slice i N) = (2 ^ 64) * valImpl (l.slice (i + 1) N) + (l.index i) := by
-    match l with
-    | h::tl => {
-      if hi : i = 0
-      then {
-        rw [hi]
-        simp only [zero_add, ne_eq, zero_ne_one, not_false_eq_true, neq_imp,
-          List.slice_nzero_cons, sub_self, List.index_zero_cons]
-        rw [List.slice]
-        simp only [sub_zero, List.idrop_zero]
-        rw [List.itake]
-        have h3 := lt_of_le_of_lt h0 h1
-        have h4 := ne_of_lt h3
-        simp only [h4, not_false_eq_true, neq_imp, ↓reduceIte]
-        rw [valImpl]
-        rw [add_comm]
-        rw [mul_comm]
-        rw [List.slice]
-        simp
-      }
-      else {
-        have hi1 : i + 1 ≠ 0 := by scalar_tac
-        simp only [ne_eq, not_false_eq_true, List.slice_nzero_cons, List.index_nzero_cons, hi, hi1]
-        rw [BigInt.slice_eq]
-        simp
-        scalar_tac
-        scalar_tac
-        simp [*] at h2
-        rw [add_comm] at h2
-        simp [*]
-      }
-    }
-    | [] => {
-      simp at h2
-      have h3 := lt_of_le_of_lt h0 h1
-      have h4 := not_le_of_lt h3
-      simp [h2] at h4
-    }
-
-lemma BigInt.mod_value_eq (n : Int) : BigInt.mod_value n = (2 ^ 64) ^ n.toNat := by
-  rw [BigInt.mod_value]
-  rw [U64.max]
-  simp
 
 lemma add_with_carry_loop_correct :
   ∀ (N : Usize) (self : Array U64 N) (other : Array U64 N) (carry : U8) (i : Usize) (h : i ≤ N),
@@ -223,7 +26,7 @@ lemma add_with_carry_loop_correct :
     rw [biginteger.BigIntegertestbigintegerBigIntN.add_with_carry_loop]
     if hind : (N.val - i.val).toNat = 0 then
       have hieqN : i = N := by {
-        simp only [Int.toNat_eq_zero, tsub_le_iff_right, zero_add] at hind;
+        simp only [Int.toNat_eq_zero, tsub_le_iff_right, zero_add] at hind; 
         simp [Scalar.le_equiv] at h
         scalar_tac
       }
@@ -235,7 +38,7 @@ lemma add_with_carry_loop_correct :
       simp [*]
     else
       have hiltN : i < N := by {
-        simp only [Int.toNat_eq_zero, tsub_le_iff_right, zero_add, not_le] at hind
+        simp only [Int.toNat_eq_zero, tsub_le_iff_right, zero_add, not_le] at hind 
         simp [Scalar.lt_equiv]
         scalar_tac
       }
@@ -311,24 +114,24 @@ decreasing_by
   scalar_tac
   simp [sub_one_lt, *]
 
-
-lemma full_itake (l : List α) (N: Int) (h : N = l.len): List.itake N l = l := by
-  unfold List.itake;
-  match hl : l with
-  | [] => simp [hl];
-  | hs::tl => {
-    if hn : N = 0 then
-      simp at h;
-      scalar_tac;
-    else
-      simp only [hn, not_false_eq_true, neq_imp, ↓reduceIte, List.cons.injEq, true_and];
-      simp [full_itake, *]
-  }
-
-lemma full_slice (l : List α) (N: Int) (h : N = l.len): List.slice 0 N l = l := by
-  unfold List.slice
-  simp only [sub_zero, List.idrop_zero]
-  simp only [full_itake, h]
+lemma add_with_carry_correct :
+  ∀ (N : Usize) (self : BigInt N) (other : BigInt N),
+  ∃ b v, biginteger.BigIntegertestbigintegerBigIntN.add_with_carry N self other = .ok (b, v) ∧
+  v.val = (self.val + other.val) % (BigInt.mod_value N.val) := by
+    intro N
+    intro self other
+    simp only [biginteger.BigIntegertestbigintegerBigIntN.add_with_carry]
+    progress with add_with_carry_loop_correct as ⟨ i, hi, hid ⟩
+    . scalar_tac
+    exists i, hi
+    simp only [true_and] 
+    unfold BigInt.mod_value at hid
+    simp only [Scalar.ofInt_val_eq, Int.toNat_zero, pow_zero, one_mul] at hid
+    have other_full_slice : List.slice 0 N.val other.v = other.v := by simp only [BigInt.len_spec, full_slice]
+    simp only [other_full_slice] at hid 
+    unfold BigInt.val
+    unfold BigInt.mod_value
+    simp [*]
 
 lemma add_with_carry_loop_overflow_correct
   (N : Usize) (self : Array U64 N) (other : Array U64 N) (carry : U8) (i : Usize)
@@ -337,9 +140,9 @@ lemma add_with_carry_loop_overflow_correct
   (b ↔ valImpl self.val + (valImpl (other.val.slice i.val N.val) + carry.val)* (BigInt.mod_value i) > BigInt.max_value N) := by
   rw [biginteger.BigIntegertestbigintegerBigIntN.add_with_carry_loop]
   if hind : (N.val - i.val).toNat = 0 then
-    have hieqN : i = N := by
+    have hieqN : i = N := by 
       {
-        simp only [Int.toNat_eq_zero, tsub_le_iff_right, zero_add] at hind;
+        simp only [Int.toNat_eq_zero, tsub_le_iff_right, zero_add] at hind; 
         simp [Scalar.le_equiv] at h
         scalar_tac
       }
@@ -351,7 +154,7 @@ lemma add_with_carry_loop_overflow_correct
     rw[List.slice]
     simp
     have he0: valImpl [] =0 :=
-     by
+     by 
      unfold valImpl
      linarith
     rw[he0]
@@ -369,15 +172,15 @@ lemma add_with_carry_loop_overflow_correct
     contrapose! h₁
     rw[h₁]
     simp
-    have hn: 0 ≤ valImpl self.val:=
+    have hn: 0 ≤ valImpl self.val:= 
      by exact valImpl_ge_zero self.val
-    have h2n: valImpl self.val < BigInt.mod_value N.val :=
+    have h2n: valImpl self.val < BigInt.mod_value N.val := 
      by exact BigInt.val_lt_mod N self
     unfold BigInt.max_value
     linarith
-  else
+  else 
    have hiltN : i < N := by {
-        simp only [Int.toNat_eq_zero, tsub_le_iff_right, zero_add, not_le] at hind
+        simp only [Int.toNat_eq_zero, tsub_le_iff_right, zero_add, not_le] at hind 
         simp [Scalar.lt_equiv]
         scalar_tac
       }
@@ -398,7 +201,7 @@ lemma add_with_carry_loop_overflow_correct
     by
     linarith
    have hdivineq : (i1.val+i2.val+carry.val)/2^64<2 :=
-    by
+    by 
      rw[Int.ediv_lt_iff_lt_mul]
      exact hii12
      linarith
@@ -445,10 +248,10 @@ lemma add_with_carry_loop_overflow_correct
    have hitn: Int.toNat 1 = 1 :=
       by simp
    have hmax:U64.max+1=2^64:=
-      by
+      by 
        .scalar_tac
    have h_pow_plus_one: (U64.max + 1) ^ Int.toNat (i.val + 1)=(U64.max + 1) ^ Int.toNat (i.val)*2^64:=
-    by
+    by 
      rw [Int.toNat_add]
      rw[pow_add]
      rw [hitn]
@@ -468,7 +271,7 @@ lemma add_with_carry_loop_overflow_correct
        by .scalar_tac
    rw[hff]
    have hmd: (i1.val + i2.val + carry.val) % 2 ^ 64 + (i1.val + i2.val + carry.val) / 2 ^ 64 * 2 ^ 64 =(i1.val + i2.val + carry.val):=
-    by
+    by 
      have hmdd:= Int.emod_add_ediv (i1.val + i2.val + carry.val) (2^64)
      .scalar_tac
    rw[hmd]
@@ -493,15 +296,7 @@ lemma add_with_carry_loop_overflow_correct
     scalar_tac
     simp [sub_one_lt, *]
 
-def bool_to_int (b:Bool) := if b then 0 else 1
-
-lemma add_with_carry_spec (N : Usize) (self : BigInt N) (other : BigInt N) :
-  ∃ b v, biginteger.BigIntegertestbigintegerBigIntN.add_with_carry N self other = .ok (b, v) ∧
-  (bool_to_int b) * (BigInt.mod_value N.val) + v.val = self.val + other.val
-  := by
-  sorry
-
-lemma add_with_carry_overflow [Inhabited U64] :
+lemma add_with_carry_overflow [Inhabited U64] : 
   ∀ (N : Usize) (self : BigInt N) (other : BigInt N),
   ∃ b val, biginteger.BigIntegertestbigintegerBigIntN.add_with_carry N self other = .ok (b, val) ∧
   (¬b ↔ self.val + other.val ≤ BigInt.max_value N) :=
@@ -520,7 +315,7 @@ by
   simp at hid
   rw [BigInt.val]
   rw [BigInt.mod_value] at hid
-  simp at hid
+  simp at hid 
   simp only [other_full_slice] at hid
   exact hid
   intro h₁
@@ -531,58 +326,14 @@ by
   simp at hid
   simp only [other_full_slice] at hid
   rw [BigInt.mod_value] at hid
-  simp at hid
+  simp at hid 
   exact hid
 
-lemma add_with_carry_correct :
-  ∀ (N : Usize) (self : BigInt N) (other : BigInt N),
+lemma add_with_carry_spec (N : Usize) (self : BigInt N) (other : BigInt N) :
   ∃ b v, biginteger.BigIntegertestbigintegerBigIntN.add_with_carry N self other = .ok (b, v) ∧
-  v.val = (self.val + other.val) % (BigInt.mod_value N.val) := by
-    intro N
-    intro self other
-    simp only [biginteger.BigIntegertestbigintegerBigIntN.add_with_carry]
-    progress with add_with_carry_loop_correct as ⟨ i, hi, hid ⟩
-    . scalar_tac
-    exists i, hi
-    simp only [true_and]
-    unfold BigInt.mod_value at hid
-    simp only [Scalar.ofInt_val_eq, Int.toNat_zero, pow_zero, one_mul] at hid
-    have other_full_slice : List.slice 0 N.val other.v = other.v := by simp only [BigInt.len_spec, full_slice]
-    simp only [other_full_slice] at hid
-    unfold BigInt.val
-    unfold BigInt.mod_value
-    simp [*]
-
-lemma is_even_correct :
-  ∀ (N : Usize) (self: BigInt N) (h: 0 < N.val),
-  ∃ b, biginteger.BigInt.const_is_even N self = .ok b ∧ b = (self.val % 2 = 0) := by {
-    intro N self h
-    unfold biginteger.BigInt.const_is_even
-    progress with Array.index_usize_spec as ⟨ idef, idecl ⟩
-    progress as ⟨ is_even_def, is_even_decl ⟩
-    simp
-    rw [Scalar.eq_equiv]
-    rw [is_even_decl]
-    rw [idecl]
-    simp [*]
-    unfold BigInt.val
-    unfold valImpl
-    match h_self : self.v with
-    | x::xs => {
-      unfold List.index
-      simp only [h_self]
-      simp only [↓reduceIte]
-      rw [Int.add_emod]
-      rw [Int.mul_emod]
-      simp
-    }
-    | [] => {
-      have h_contr := BigInt.len_spec N self
-      simp [h_self] at h_contr
-      rw [←h_contr] at h
-      simp at h
-    }
-  }
+  (bool_to_int b) * (BigInt.mod_value N.val) + v.val = self.val + other.val
+  := by
+  sorry
 
 end biginteger
 
