test/lean/Common/Base.lean
@@ -1,0 +1,201 @@
+import Test.Funs
+import Base
+
+open Primitives
+open Result
+
+namespace test
+
+namespace biginteger
+
+attribute [-simp] Bool.exists_bool
+
+def valImpl (l : List U64) : Int :=
+  match l with
+  | a::b => a.val + (valImpl b) * (2 ^ 64)
+  | [] => 0
+
+lemma valImpl_ge_zero (l : List U64) : valImpl l ≥ 0 := by
+  unfold valImpl
+  match l with
+  | a::b => {
+    have ha : 0 ≤ a.val := by scalar_tac
+    have hb : 0 ≤ valImpl b * 2 ^ 64 := by simp[valImpl_ge_zero]
+    have hc := Int.add_le_add ha hb
+    simp at hc
+    simp [*]
+  }
+  | [] => simp
+
+@[simp]
+lemma tmp : Inhabited U64 := by
+  constructor
+  apply 0#u64
+
+-- Biggest part by Son Ho
+lemma BigInt.update_eq (l : List U64) (i : Int) (x : U64)
+  (h0 : 0 ≤ i) (h1 : i < l.len) :
+  valImpl (l.update i x) = valImpl l + (x - l.index i) * ((2 ^ 64) ^ i.toNat) := by
+  match l with
+  | [] =>
+    -- Contradiction: 0 ≤ i ∧ i < 0
+    simp at h1
+    scalar_tac
+  | h :: tl =>
+    simp at h1
+    if i = 0 then
+      simp [*] -- By writing [*] I'm using the hypothesis i = 0
+      unfold valImpl
+      scalar_tac
+    else
+      have hnz : i ≠ 0 := by scalar_tac
+      -- This uses update_nzero_cons and index_nzero_cons
+      simp only [h1, hnz, ne_eq, not_false_eq_true, List.update_nzero_cons, List.index_nzero_cons] -- By writing [*] I'm using the hypothesis i ≠ 0
+      unfold valImpl
+      -- Recursive call
+      have heq := update_eq tl (i - 1) x (by scalar_tac) (by scalar_tac)
+      rw [heq]
+      rw [add_mul]
+      simp only [Int.pred_toNat]
+      have hexpr : ((2: Int) ^ 64) ^ (Int.toNat i - 1) * 2 ^ 64 = (2 ^ 64) ^ Int.toNat i := by {
+        rw [←pow_mul]
+        rw [←pow_add]
+        rw [←pow_mul]
+        rw [Nat.mul_sub_left_distrib]
+        rw [←Nat.sub_add_comm]
+        simp [*]
+        have hgone : i ≥ 1 := by scalar_tac
+        simp [hgone, *]
+      }
+      simp only [mul_assoc]
+      rw [hexpr]
+      simp [add_assoc]
+
+
+@[simp] lemma BigInt.len_spec
+  (N : Usize) (self : biginteger.BigInt N) :
+  (self.val).len = N.val := by
+  have h := self.property
+  rw [List.len_eq_length]
+  apply h
+
+def BigInt.val {N : Usize} (x : biginteger.BigInt N) : Int := valImpl x.v
+
+def BigInt.mod_value (n : Int) : Int := (U64.max + 1) ^ (Int.toNat n)
+
+def BigInt.max_value (n : Int) : Int := BigInt.mod_value n - 1
+
+lemma BigInt.mod_value_add_one (n : Int) (hn : 0 ≤ n) : BigInt.mod_value n * (2 ^ 64) = BigInt.mod_value (n + 1) := by
+  rw [BigInt.mod_value]
+  rw [BigInt.mod_value]
+  rw [U64.max]
+  simp
+  -- rw [mul_comm]
+  rw [←pow_succ]
+  -- simp []
+  have hf := Int.toNat_add_nat hn 1
+  rw [←hf]
+  simp
+
+lemma valImpl_lt_mod (l : List U64) : valImpl l < BigInt.mod_value l.len := by
+  unfold valImpl
+  match h : l with
+  | a::b => {
+    simp only [List.len_cons, gt_iff_lt]
+    have ha := valImpl_lt_mod b
+    have hb : a.val < 2 ^ 64 := by scalar_tac
+    have hc := Int.le_sub_one_of_lt ha
+    have hd : 1 + b.len = b.len + 1 := by scalar_tac
+    have hf : (0 : Int) ≤ 2 ^ 64 := by simp 
+    have hg := Int.mul_le_mul_of_nonneg_right hc hf
+    simp only [Int.sub_mul] at hg
+    simp only [one_mul] at hg
+    have hh := add_lt_add_of_le_of_lt hg hb
+    simp only [sub_add_cancel] at hh
+    rw [Int.add_comm] at hh
+    rw [hd]
+    rw [←BigInt.mod_value_add_one]
+    simp only [hh]
+    scalar_tac
+  }
+  | [] => {
+    simp
+    unfold BigInt.mod_value
+    simp
+  }
+
+lemma BigInt.val_lt_mod (N : Usize) (bn : Array U64 N) : valImpl bn.val < BigInt.mod_value N.val := by
+  have hi := valImpl_lt_mod bn.val
+  have he := bn.property
+  simp [*, List.len_eq_length] at hi
+  simp [*]
+
+lemma BigInt.slice_eq (l : List U64) (i : Int) (N : Int)
+  (h0 : 0 ≤ i) (h1 : i < N) (h2 : N ≤ l.len) :
+  valImpl (l.slice i N) = (2 ^ 64) * valImpl (l.slice (i + 1) N) + (l.index i) := by
+    match l with
+    | h::tl => {
+      if hi : i = 0
+      then {
+        rw [hi]
+        simp only [zero_add, ne_eq, zero_ne_one, not_false_eq_true, neq_imp,
+          List.slice_nzero_cons, sub_self, List.index_zero_cons]
+        rw [List.slice]
+        simp only [sub_zero, List.idrop_zero]
+        rw [List.itake]
+        have h3 := lt_of_le_of_lt h0 h1
+        have h4 := ne_of_lt h3
+        simp only [h4, not_false_eq_true, neq_imp, ↓reduceIte]
+        rw [valImpl]
+        rw [add_comm]
+        rw [mul_comm]
+        rw [List.slice]
+        simp
+      }
+      else {
+        have hi1 : i + 1 ≠ 0 := by scalar_tac
+        simp only [ne_eq, not_false_eq_true, List.slice_nzero_cons, List.index_nzero_cons, hi, hi1]
+        rw [BigInt.slice_eq]
+        simp
+        scalar_tac
+        scalar_tac
+        simp [*] at h2
+        rw [add_comm] at h2
+        simp [*]
+      }
+    }
+    | [] => {
+      simp at h2
+      have h3 := lt_of_le_of_lt h0 h1
+      have h4 := not_le_of_lt h3
+      simp [h2] at h4
+    }
+
+lemma BigInt.mod_value_eq (n : Int) : BigInt.mod_value n = (2 ^ 64) ^ n.toNat := by
+  rw [BigInt.mod_value]
+  rw [U64.max]
+  simp
+
+lemma full_itake (l : List α) (N: Int) (h : N = l.len): List.itake N l = l := by
+  unfold List.itake;
+  match hl : l with
+  | [] => simp [hl];
+  | hs::tl => {
+    if hn : N = 0 then
+      simp at h;
+      scalar_tac;
+    else
+      simp only [hn, not_false_eq_true, neq_imp, ↓reduceIte, List.cons.injEq, true_and];
+      simp [full_itake, *]
+  }
+
+lemma full_slice (l : List α) (N: Int) (h : N = l.len): List.slice 0 N l = l := by
+  unfold List.slice
+  simp only [sub_zero, List.idrop_zero]
+  simp only [full_itake, h]
+
+def bool_to_int (b:Bool) := if b then 0 else 1
+
+end biginteger
+
+end test
