test/lean/lakefile.lean
@@ -11,6 +11,14 @@ lean_lib «Test» {
   -- add library configuration options here
 }
 
+lean_lib «Common» {
+  -- add library configuration options here
+}
+
+lean_lib «Proofs» {
+  -- add library configuration options here
+}
+
 @[default_target]
 lean_exe «test» {
   root := `Proofs
